lib/Util.v
@@ -167,138 +167,28 @@ Section Forall2.
   Qed.
 End Forall2.
 
-(** List helpers. *)
-
-Section List.
-  Context {A : Set}.
-
-  Fixpoint Has (a : A) (Γ : list A) : Set :=
-    match Γ with
-    | []    => Empty_set
-    | h :: Δ => ((h = a) + Has a Δ)%type
-    end.
-
-  Variant zilch : list A -> Prop := zilch_nil : zilch [].
+Section AccLemmas.
+  Local Hint Constructors Acc : core.
   
-  Definition lookup :
-    forall {Γ : list A} {n : nat},
-      n < length Γ -> A.
+  Lemma acc_pres : forall A B (f : A -> B) (R : A -> A -> Prop) (Q : B -> B -> Prop),
+    (forall a1 a2, R a1 a2 -> Q (f a1) (f a2)) ->
+    forall a, Acc Q (f a) -> Acc R a.
   Proof.
-    refine
-      (fix F Γ n HnΓ :=
-         match Γ as Γ' return Γ = Γ' -> A with
-         | []
-           => fun HΓΓ' => _
-         | a :: Δ
-         => fun HΓΓ' =>
-             match n as n' return n = n' -> A with
-             | O   => fun _ => a
-             | S k => fun Hnn' => F Δ k _
-             end eq_refl
-         end eq_refl).
-    - inv HΓΓ'; cbn in *; lia.
-    - subst; cbn in *; lia.
-  Defined.
-  
-  (* Require Import Extraction.
-     Recursive Extraction lookup. *)
+    intros A B f R Q Hmap a HQ.
+    remember (f a) as fa eqn:Heqfa.
+    generalize dependent a.
+    induction HQ; intros a Heqfa; subst; eauto.
+  Qed.
 
-  Definition length_nth_error' :
-    forall {l : list A} {n : nat},
-      n < length l -> { a | nth_error l n = Some a }.
+  Lemma Acc_ind2 :
+    forall A B (RA : A -> A -> Prop) (RB : B -> B -> Prop) (P : A -> B -> Prop),
+      (forall a b, (forall a', RA a' a -> P a' b) ->
+              (forall b', RB b' b -> P a b') -> P a b) ->
+      forall a b, Acc RA a -> Acc RB b -> P a b.
   Proof.
-    refine
-    (fix F l n Hnl :=
-       match
-         l as l'
-         return
-         l = l' -> { a | nth_error l n = Some a } with
-       | [] => fun H => _
-       | h :: t
-         => fun H =>
-             match
-               n as n'
-               return
-               n = n' -> { a | nth_error l n = Some a } with
-             | O
-               => fun _ => @exist _ _ h _
-             | S k
-               => fun Hnn' =>
-                   match F t k _ with
-                   | exist _ a' Hk => @exist _ _ a' _
-                   end
-             end eq_refl
-       end eq_refl); subst; cbn in *;
-      lia || reflexivity || assumption.
-  Defined.
-
-
-  Definition nth_error_lookup :
-    forall {Γ : list A} {n : nat} (H : n < length Γ),
-      nth_error Γ n = Some (lookup H).
-  Proof.
-    intro l; induction l as [| a l IHl];
-      intros [| n] H; cbn in *;
-        try lia; eauto using Lt.lt_S_n.
-  Defined.
-
-  Definition ext' : forall {Γ Δ},
-      (forall a, Has a Γ -> Has a Δ) ->
-      forall b a, Has a (b :: Γ) -> Has a (b :: Δ).
-  Proof.
-    refine
-      (fun l d f b a H =>
-         match l as l' return l = l' -> Has a (b :: d) with
-         | [] => fun Hl => inl _
-         | h :: t
-           => fun Hl =>
-               match H with
-               | inl Hh => inl Hh
-               | inr Ht => inr (f _ Ht)
-               end
-         end eq_refl); subst; cbn in *.
-    destruct H as [H | H]; subst; reflexivity || contradiction.
-  Defined.
-
-  Definition Has_nth_error : forall {Γ a},
-      Has a Γ -> { n | nth_error Γ n = Some a}.
-  Proof.
-    intro l; induction l as [| h t IHt];
-      intros a Hal; cbn in *; try contradiction.
-    destruct Hal as [Hha | Hat]; subst.
-    - refine (exist _ 0 _); reflexivity.
-    - apply IHt in Hat as [k Hk].
-      refine (exist _ (S k) _); assumption.
-  Defined.
-
-  Definition nth_error_Has : forall {Γ a n},
-      nth_error Γ n = Some a -> Has a Γ.
-  Proof.
-    intro l; induction l as [| h t IHt];
-      intros a [| n] Hnth; cbn in *; try discriminate.
-    - inv Hnth; left; reflexivity.
-    - apply IHt in Hnth; right; assumption.
-  Defined.
-
-  Definition nth_error_Has' : forall {Γ a},
-      {n | nth_error Γ n = Some a} -> Has a Γ.
-  Proof.
-    intros l a [n H]; exact (nth_error_Has H).
-  Defined.
-
-  Fail Definition nth_error_Has : forall {Γ a},
-      Has a Γ <-> {n | nth_error Γ n = Some a}.
-  
-  Definition ext : forall {Γ Δ : list A},
-      (forall a, {n | nth_error Γ n = Some a} ->
-              {k | nth_error Δ k = Some a}) ->
-      forall b a, {n | nth_error (b :: Γ) n = Some a} ->
-               {k | nth_error (b :: Δ) k = Some a}.
-  Proof.
-    intros l d f b a Hab.
-    apply Has_nth_error.
-    apply nth_error_Has' in Hab.
-    pose proof (fun a H => nth_error_Has' (f a (Has_nth_error H))) as H.
-    eauto using ext'.
-  Defined.
-End List.
+    intros A B R Q P H a b HA.
+    generalize dependent b.
+    induction HA; intros b HB;
+      induction HB; eauto.
+  Qed.
+End AccLemmas.
