lib/ListUtil.v
@@ -1,0 +1,162 @@
+Require Export Lambda.Util.
+From Equations Require Export Equations.
+
+(** * List helpers. *)
+
+Section List.
+  Context {A : Set}.
+
+  Inductive Has : A -> list A -> Set :=
+  | HasO : forall a t, Has a (a :: t)
+  | HasS : forall a h t, Has a t -> Has a (h :: t).
+
+  Global Arguments HasO {_} {_}.
+  Global Arguments HasS {_} {_} {_}.
+
+  Equations Derive NoConfusion NoConfusionHom Subterm for list.
+  Equations Derive Signature NoConfusion for Has.
+  (*Equations Derive NoConfusionHom for Has.*)
+  (*Next Obligation.
+  Proof.
+    unfold NoConfusionHom_Has in H.
+    unfold apply_noConfusion in H. cbn in H.
+    unfold DepElim.solution_left,DepElim.solution_right in H.
+    unfold DepElim.eq_simplification_sigma1,Logic.transport in H.
+    repeat unfold noConfusionHom_list_obligation_2,
+      noConfusionHom_list_obligation_4,
+      noConfusionHom_list_obligation_1,
+      NoConfusionHom_list,eq_sym in H. cbn in H.
+    depind a0; cbn in *; depelim b; cbn in *.
+    - unfold DepElim.pack_sigma_eq_nondep in *.
+      Search (eq_rect (_ :: _) _ _ (_ :: _) _).
+      rewrite f_equal_dep in H.
+      Print Assumptions Eqdep.EqdepTheory.eq_rect_eq.
+      depelim e'; cbn in *. inv H.
+      depelim e'0; cbn in *.
+    - admit.
+    - admit.
+    - f_equal.*)
+
+  Equations ext_has : forall {Γ Δ},
+      (forall {a : A}, Has a Γ -> Has a Δ) ->
+      forall {b a : A}, Has a (b :: Γ) -> Has a (b :: Δ) :=
+    ext_has ρ HasO := HasO;
+    ext_has ρ (HasS h) := HasS (ρ _ h).
+  
+  Definition Has_nth_error : forall {Γ a},
+      Has a Γ -> { n | nth_error Γ n = Some a}.
+  Proof.
+    intros l a h; induction h.
+    - refine (exist _ 0 _); reflexivity.
+    - destruct IHh as [k Hk].
+      refine (exist _ (S k) _); assumption.
+  Defined.
+  
+  Variant zilch : list A -> Prop := zilch_nil : zilch [].
+  
+  Definition lookup :
+    forall {Γ : list A} {n : nat},
+      n < length Γ -> A.
+  Proof.
+    refine
+      (fix F Γ n HnΓ :=
+         match Γ as Γ' return Γ = Γ' -> A with
+         | []
+           => fun HΓΓ' => _
+         | a :: Δ
+         => fun HΓΓ' =>
+             match n as n' return n = n' -> A with
+             | O   => fun _ => a
+             | S k => fun Hnn' => F Δ k _
+             end eq_refl
+         end eq_refl).
+    - inv HΓΓ'; cbn in *; lia.
+    - subst; cbn in *; lia.
+  Defined.
+  
+  (* Require Import Extraction.
+     Recursive Extraction lookup. *)
+
+  Definition length_nth_error' :
+    forall {l : list A} {n : nat},
+      n < length l -> { a | nth_error l n = Some a }.
+  Proof.
+    refine
+    (fix F l n Hnl :=
+       match
+         l as l'
+         return
+         l = l' -> { a | nth_error l n = Some a } with
+       | [] => fun H => _
+       | h :: t
+         => fun H =>
+             match
+               n as n'
+               return
+               n = n' -> { a | nth_error l n = Some a } with
+             | O
+               => fun _ => @exist _ _ h _
+             | S k
+               => fun Hnn' =>
+                   match F t k _ with
+                   | exist _ a' Hk => @exist _ _ a' _
+                   end
+             end eq_refl
+       end eq_refl); subst; cbn in *;
+      lia || reflexivity || assumption.
+  Defined.
+
+  Definition nth_error_lookup :
+    forall {Γ : list A} {n : nat} (H : n < length Γ),
+      nth_error Γ n = Some (lookup H).
+  Proof.
+    intro l; induction l as [| a l IHl];
+      intros [| n] H; cbn in *;
+        try lia; eauto using Lt.lt_S_n.
+  Defined.
+
+  Local Hint Constructors Has : core.
+  
+  Definition nth_error_Has : forall {Γ a n},
+      nth_error Γ n = Some a -> Has a Γ.
+  Proof.
+    intro l; induction l as [| h t IHt];
+      intros a [| n] Hnth; cbn in *; try discriminate; eauto.
+    inv Hnth; auto.
+  Defined.
+
+  Definition nth_error_Has' : forall {Γ a},
+      {n | nth_error Γ n = Some a} -> Has a Γ.
+  Proof.
+    intros l a [n H]; exact (nth_error_Has H).
+  Defined.
+  
+  Definition ext_nth_error : forall {Γ Δ : list A},
+      (forall a, {n | nth_error Γ n = Some a} ->
+              {k | nth_error Δ k = Some a}) ->
+      forall b a, {n | nth_error (b :: Γ) n = Some a} ->
+               {k | nth_error (b :: Δ) k = Some a}.
+  Proof.
+    intros l d f b a Hab.
+    apply Has_nth_error.
+    apply nth_error_Has' in Hab.
+    pose proof (fun a H => nth_error_Has' (f a (Has_nth_error H))) as H.
+    eauto using ext_has.
+  Defined.
+End List.
+
+Equations has_map :
+  forall {A B : Set} (f : A -> B) {l : list A} {e : A},
+    Has e l -> Has (f e) (map f l) :=
+  has_map f  HasO     := HasO;
+  has_map f (HasS hs) := HasS (has_map f hs).
+
+Definition map_has : forall (A B : Set) (f : A -> B) (l : list A) b,
+    Has b (map f l) -> {a : A & f a = b & Has a l}.
+Proof.
+  intros A B f l.
+  induction l as [| a l ih]; intros b h; cbn in *; depelim h.
+  - exact (existT2 _ _ a eq_refl HasO).
+  - apply ih in h0 as [a' fab hasa].
+    exact (existT2 _ _ a' fab (HasS hasa)).
+Defined.
