lib/STLC/Has.v
@@ -1,5 +1,4 @@
-Require Export Lambda.STLC.SimpleTypes.
-From Equations Require Import Equations.
+From Lambda Require Export ListUtil STLC.SimpleTypes.
 
 (** Inspired by
     Programming Language Foundations in Agda. *)
@@ -23,3 +22,41 @@ where "Γ '⊢' τ" := (term Γ τ) : type_scope.
 
 Derive Signature for term.
 Equations Derive NoConfusion NoConfusionHom Subterm for term.
+
+Declare Scope term_scope.
+Delimit Scope term_scope with term.
+
+Notation "'`λ' t"
+  := (Abs _ _ _ t)
+       (at level 15, right associativity) : term_scope.
+Notation "'λ' τ '⇒' t"
+  := (Abs _ τ _ t)
+       (at level 15, right associativity) : term_scope.
+Notation "'λ' τ '↣' .. '↣' ρ '⇒' t"
+  := (Abs _ τ _ .. (Abs _ ρ _ t) ..)
+       (at level 15, right associativity) : term_scope.
+Notation "x '⋅' y"
+  := (App _ _ _ x y)
+       (at level 14, left associativity) : term_scope.
+
+Equations
+  Rename
+  {Γ Δ} :
+  (forall {τ}, Has τ Γ -> Has τ Δ) -> forall {σ}, Γ ⊢ σ -> Δ ⊢ σ :=
+  Rename f (Id _ _ h)   := Id _ _ (f _ h);
+  Rename f (λ ρ ⇒ t')%term := (`λ Rename (@ext_has _ _ _ f ρ) t')%term;
+  Rename f (t₁ ⋅ t₂)%term  := (Rename f t₁ ⋅ Rename f t₂)%term.
+
+Equations Exts : forall {Γ Δ},
+    (forall {τ}, Has τ Γ -> Δ ⊢ τ) ->
+    forall ρ {σ}, Has σ (ρ :: Γ) -> ρ :: Δ ⊢ σ :=
+  Exts f _ HasO := Id _ _ HasO;
+  Exts f _ (HasS hs) := Rename (fun τ => @HasS _ τ _ _) (f _ hs).
+
+Equations
+  subs : forall {Γ Δ},
+    (forall {τ}, Has τ Γ -> Δ ⊢ τ) ->
+    forall {σ}, Γ ⊢ σ -> Δ ⊢ σ :=
+  subs f (Id _ _ h)   := f _ h;
+  subs f (λ ρ ⇒ t')%term := (`λ subs (fun τ => Exts f ρ (σ:=τ)) t')%term;
+  subs f (t₁ ⋅ t₂)%term  := (subs f t₁ ⋅ subs f t₂)%term.
